src/PermDiskLog.v
@@ -1,0 +1,257 @@
+Require Import Arith.
+Require Import Bool.
+Require Import Eqdep_dec.
+Require Import Classes.SetoidTactics.
+Require Import PermHashmap.
+Require Import HashmapProg.
+Require Import Pred PermPredCrash.
+Require Import Omega.
+Require Import Word.
+Require Import Rec.
+Require Import WordAuto.
+Require Import FSLayout.
+Require Import Rounding.
+Require Import List ListUtils.
+Require Import Psatz.
+Require Import PermAsyncRecArray.
+Require Export PermDiskLogHdr.
+
+Set Implicit Arguments.
+
+Definition entry := (addr * tagged_block)%type.
+Definition contents := list entry.
+
+Inductive state :=
+(* The log is synced on disk *)
+| Synced (l: contents)
+         
+(* The log has been truncated; but the length (0) is unsynced *)
+| Truncated (old: contents)
+            
+(* The log is being extended; only the content has been updated (unsynced) *)
+| Extended (old: contents) (new: contents)
+           
+(* The log immediately after a crash during an extend, when the new header
+  gets synced to disk, but we're not sure what data is there yet. This state
+  should be hidden from all higher layers. *)
+| ExtendedCrashed (old: contents) (new: contents)
+                  
+(* A special case of ExtendedCrashed. The data in the log definitely does
+  not match the header on disk, so we are guaranteed to roll back to the
+  previous length during recovery. *)
+| Rollback (old: contents)
+           
+(* The log during recovery, when the data in the log doesn't match the
+  header and we're rolling back to the previous log length. The header we will
+  recover to hasn't been synced yet *)
+| RollbackUnsync (old: contents)
+.
+
+Definition ent_addr (e : entry) := addr2w (fst e).
+Definition ent_tag (e : entry) := fst (snd e).
+Definition ent_valu (e : entry) := snd (snd e).
+
+Definition ndesc_log (log : contents) := (divup (length log) DescSig.items_per_val).
+Definition ndesc_list T (l : list T) := (divup (length l) DescSig.items_per_val).
+
+Fixpoint log_nonzero (log : contents) : list entry :=
+  match log with
+  | (0, _) :: rest => log_nonzero rest
+  | e :: rest => e :: log_nonzero rest
+  | nil => nil
+  end.
+
+Definition vals_nonzero (log : contents) := map ent_valu (log_nonzero log).
+Definition tags_nonzero (log : contents) := map ent_tag (log_nonzero log).
+
+Fixpoint nonzero_addrs (al : list addr) : nat :=
+  match al with
+  | 0 :: rest => nonzero_addrs rest
+  | e :: rest => S (nonzero_addrs rest)
+  | nil => 0
+  end.
+
+Fixpoint combine_nonzero (al : list addr) (vl : list tagged_block) : contents :=
+  match al, vl with
+  | 0 :: al', v :: vl' => combine_nonzero al' vl
+  | a :: al', v :: vl' => (a, v) :: (combine_nonzero al' vl')
+  | _, _ => nil
+  end.
+
+Definition ndata_log (log : contents) := nonzero_addrs (map fst log) .
+
+Definition addr_valid (e : entry) := goodSize addrlen (fst e).
+
+Definition entry_valid (ent : entry) := fst ent <> 0 /\ addr_valid ent.
+
+Definition rep_contents xp (log : contents) : rawpred :=
+  ( [[ Forall addr_valid log ]] *
+    Desc.array_rep xp 0 (Desc.Synced (map ent_tag log) (map ent_addr log)) *
+    Data.array_rep xp 0 (Data.Synced (tags_nonzero log) (vals_nonzero log)) *
+    Desc.avail_rep xp (ndesc_log log) (LogDescLen xp - (ndesc_log log)) *
+    Data.avail_rep xp (ndata_log log) (LogLen xp - (ndata_log log))
+  )%pred.
+
+Definition padded_addr (al : list addr) :=
+  setlen al (roundup (length al) DescSig.items_per_val) 0.
+
+Definition padded_log (log : contents) :=
+  setlen log (roundup (length log) DescSig.items_per_val) (0, tagged_block0).
+
+Definition rep_contents_unmatched xp (old : contents) new_addr new_tag new_valu : rawpred :=
+  ( [[ Forall addr_valid old ]] *
+    (*[[ Forall addr_valid new ]] **)
+    Desc.array_rep xp 0 (Desc.Synced (map ent_tag (padded_log old))
+                                     (map ent_addr (padded_log old))) *
+    Desc.array_rep xp (ndesc_log old) (Desc.Synced new_tag new_addr) *
+    Data.array_rep xp 0 (Data.Synced (tags_nonzero (padded_log old))
+                                     (vals_nonzero (padded_log old))) *
+    Data.array_rep xp (ndata_log old) (Data.Synced new_tag new_valu) *
+    Desc.avail_rep xp (ndesc_log old + ndesc_list new_addr)
+                   (LogDescLen xp - (ndesc_log old) - (ndesc_list new_addr)) *
+    Data.avail_rep xp (ndata_log old + length new_valu)
+                   (LogLen xp - (ndata_log old) - (length new_valu))
+  )%pred.
+
+Definition loglen_valid xp ndesc ndata :=
+  ndesc <= LogDescLen xp  /\ ndata <= LogLen xp.
+
+Definition loglen_invalid xp ndesc ndata :=
+  ndesc > LogDescLen xp \/ ndata > LogLen xp.
+
+Definition checksums_match (l : contents) h hm :=
+  hash_list_rep (rev (DescDefs.ipack (map ent_addr l))) (fst h) hm /\
+  hash_list_rep (rev (vals_nonzero l)) (snd h) hm.
+
+Definition hide_or (P : Prop) := P.
+Opaque hide_or.
+
+Definition rep_inner xp (st : state) hm : rawpred :=
+  (match st with
+   | Synced l =>
+     exists prev_len h,
+     Hdr.rep xp (Hdr.Synced (prev_len,
+                             (ndesc_log l, ndata_log l),
+                             h)) *
+     rep_contents xp l *
+     [[ checksums_match l h hm ]]
+       
+   | Truncated old =>
+     exists prev_len h h',
+     Hdr.rep xp (Hdr.Unsync ((ndesc_log old, ndata_log old), (0, 0), h')
+                            (prev_len, (ndesc_log old, ndata_log old), h)) *
+     rep_contents xp old *
+     [[ checksums_match old h hm ]] *
+     [[ checksums_match [] h' hm ]]
+       
+   | Extended old new =>
+     exists prev_len h h',
+     Hdr.rep xp (Hdr.Unsync ((ndesc_log old, ndata_log old),
+                             (ndesc_log old + ndesc_log new,
+                              ndata_log old + ndata_log new), h')
+                            (prev_len, (ndesc_log old, ndata_log old), h)) *
+     rep_contents xp old *
+     [[ loglen_valid xp (ndesc_log old + ndesc_log new)
+                     (ndata_log old + ndata_log new) ]] *
+     [[ checksums_match old h hm ]] *
+     [[ checksums_match (padded_log old ++ new) h' hm ]] *
+     [[ Forall entry_valid new ]]
+       
+   | ExtendedCrashed old new =>
+     exists h synced_addr synced_valu ndesc,
+     Hdr.rep xp (Hdr.Synced ((ndesc_log old, ndata_log old),
+                             (ndesc_log old + ndesc_log new,
+                              ndata_log old + ndata_log new),
+                             h)) *
+     rep_contents_unmatched xp old synced_addr synced_valu *
+     [[ loglen_valid xp (ndesc_log old + ndesc_log new)
+                     (ndata_log old + ndata_log new) ]] *
+     (* Whatever got synced on disk takes up just as many desc blocks as new should've. *)
+     [[ length synced_addr = (ndesc * DescSig.items_per_val)%nat ]] *
+     [[ ndesc = ndesc_log new ]] *
+     [[ length synced_valu = ndata_log new ]] *
+     [[ checksums_match (padded_log old ++ new) h hm ]] *
+     [[ Forall entry_valid new ]]
+       
+   | Rollback old =>
+     exists synced_addr synced_valu h new,
+     Hdr.rep xp (Hdr.Synced ((ndesc_log old, ndata_log old),
+                             (ndesc_log old + ndesc_log new,
+                              ndata_log old + ndata_log new),
+                             h)) *
+     rep_contents_unmatched xp old synced_addr synced_valu *
+     [[ loglen_valid xp (ndesc_log old + ndesc_log new)
+                     (ndata_log old + ndata_log new) ]] *
+     (* Whatever got synced on disk takes up just as many desc blocks as new should've. *)
+     [[ length synced_addr = ((ndesc_log new) * DescSig.items_per_val)%nat ]] *
+     [[ length synced_valu = ndata_log new ]] *
+     [[ checksums_match (padded_log old ++ new) h hm ]] *
+     [[ hide_or (DescDefs.ipack (map ent_addr (padded_log new)) <> DescDefs.ipack synced_addr \/
+                 vals_nonzero new <> synced_valu) ]] *
+     [[ Forall entry_valid new ]]
+       
+  | RollbackUnsync old =>
+    exists synced_addr synced_valu h h' new prev_len,
+    Hdr.rep xp (Hdr.Unsync (prev_len, (ndesc_log old, ndata_log old), h')
+                           ((ndesc_log old, ndata_log old),
+                            (ndesc_log old + ndesc_log new,
+                             ndata_log old + ndata_log new), h)) *
+    rep_contents_unmatched xp old synced_addr synced_valu *
+    [[ loglen_valid xp (ndesc_log old + ndesc_log new)
+                    (ndata_log old + ndata_log new) ]] *
+    (* Whatever got synced on disk takes up just as many desc blocks as new should've. *)
+    [[ length synced_addr = ((ndesc_log new) * DescSig.items_per_val)%nat ]] *
+    [[ length synced_valu = ndata_log new ]] *
+    [[ checksums_match old h' hm ]] *
+    [[ checksums_match (padded_log old ++ new) h hm ]] *
+    [[ hide_or (DescDefs.ipack (map ent_addr (padded_log new)) <> DescDefs.ipack synced_addr \/
+                vals_nonzero new <> synced_valu) ]] *
+    [[ Forall entry_valid new ]]
+      
+   end)%pred.
+
+Definition xparams_ok xp := 
+  DescSig.xparams_ok xp /\ DataSig.xparams_ok xp /\
+  (LogLen xp) = DescSig.items_per_val * (LogDescLen xp).
+
+Definition rep xp st hm:=
+  ([[ xparams_ok xp ]] * rep_inner xp st hm)%pred.
+
+Definition would_recover' xp l hm :=
+  (rep xp (Synced l) hm \/
+   rep xp (Rollback l) hm \/
+   rep xp (RollbackUnsync l) hm)%pred.
+
+Definition would_recover xp F l hm :=
+  (exists cs d,
+     BUFCACHE.rep cs d *
+     [[ (F * would_recover' xp l hm)%pred d ]])%pred.
+
+
+Theorem sync_invariant_rep :
+  forall xp st hm,
+    sync_invariant (rep xp st hm).
+Proof.
+  unfold rep, rep_inner, rep_contents, rep_contents_unmatched.
+  destruct st; intros; eauto 50.
+Qed.
+
+Hint Resolve sync_invariant_rep.
+
+Theorem sync_invariant_would_recover' :
+  forall xp l hm,
+    sync_invariant (would_recover' xp l hm).
+Proof.
+  unfold would_recover'; intros; eauto.
+Qed.
+
+Theorem sync_invariant_would_recover :
+  forall xp F l hm,
+    sync_invariant (would_recover xp F l hm).
+Proof.
+  unfold would_recover; intros; eauto.
+Qed.
+
+Hint Resolve sync_invariant_would_recover sync_invariant_would_recover'.
+
+Local Hint Unfold rep rep_inner rep_contents xparams_ok: hoare_unfold.
